src/goose_lang/lang.v
@@ -104,22 +104,17 @@ Inductive prim_op0 : Type :=
 .
 
 Inductive prim_op1 : Set :=
-  | PrepareWriteOp (* loc *)
-  (* non-atomic loads (which conflict with stores) *)
-  | StartReadOp (* loc *)
-  | FinishReadOp (* loc *)
-  (* atomic loads (which still conflict with non-atomic stores) *)
-  | LoadOp
-  | InputOp
-  | OutputOp
+| PrepareWriteOp (* loc *)
+(* non-atomic loads (which conflict with stores) *)
+| StartReadOp (* loc *)
+| FinishReadOp (* loc *)
+(* atomic loads (which still conflict with non-atomic stores) *)
+| LoadOp
+| AllocOp (* initial value *)
 .
 
 Inductive prim_op2 : Set :=
- | AllocNOp (* array length (positive number), initial value *)
- | FinishStoreOp (* pointer, value *)
- | AtomicSwapOp (* pointer, value; returns old value *)
- | AtomicOpOp (op : bin_op) (* pointer, value *) (* atomic binary operation *)
- | GlobalPutOp (* string, val *)
+| FinishStoreOp (* pointer, value *)
 .
 
 Inductive arity : Set := args0 | args1 | args2.
@@ -239,27 +234,18 @@ Inductive expr :=
 | Var (x : string)
 | Rec (f x : binder) (e : expr)
 | App (e1 e2 : expr)
-(* Base types and their operations *)
-| UnOp (op : un_op) (e : expr)
-| BinOp (op : bin_op) (e1 e2 : expr)
 | If (e0 e1 e2 : expr)
 (* Products *)
 | Pair (e1 e2 : expr)
 | Fst (e : expr)
 | Snd (e : expr)
-(* Sums *)
-| InjL (e : expr)
-| InjR (e : expr)
-| Case (e0 : expr) (e1 : expr) (e2 : expr)
 (* Concurrency *)
 | Fork (e : expr)
-| Atomically (e: expr) (e : expr)
 (* Heap-based primitives *)
 | Primitive0 (op: prim_op args0)
 | Primitive1 (op: prim_op args1) (e : expr)
 | Primitive2 (op: prim_op args2) (e1 e2 : expr)
 (* | Primitive3 (op: prim_op args3) (e0 e1 e2 : expr) *)
-| CmpXchg (e0 : expr) (e1 : expr) (e2 : expr) (* Compare-exchange *)
 (* External FFI operation *)
 | ExternalOp (op: ffi_opcode) (e: expr)
 (* Prophecy *)
@@ -322,39 +308,17 @@ Bind Scope val_scope with val.
 
 Notation Panic s := (Primitive0 (PanicOp s)).
 Notation ArbitraryInt := (Primitive0 ArbitraryIntOp).
-Notation AllocN := (Primitive2 AllocNOp).
+Notation Alloc := (Primitive1 AllocOp).
 Notation PrepareWrite := (Primitive1 PrepareWriteOp).
 Notation FinishStore := (Primitive2 FinishStoreOp).
-Notation AtomicSwap := (Primitive2 AtomicSwapOp).
-Notation AtomicOp o := (Primitive2 (AtomicOpOp o)).
 Notation StartRead := (Primitive1 StartReadOp).
 Notation FinishRead := (Primitive1 FinishReadOp).
 Notation Load := (Primitive1 LoadOp).
-Notation Input := (Primitive1 InputOp).
-Notation Output := (Primitive1 OutputOp).
 
 Delimit Scope expr_scope with E.
 Delimit Scope val_scope with V.
 
 Global Open Scope Z. (* Make sure everyone gets this scope. *)
-
-Coercion LitBool : bool >-> base_lit.
-Coercion LitLoc : loc >-> base_lit.
-(* TODO: this should be added *)
-(* Coercion LitString : string >-> base_lit. *)
-Coercion LitInt : u64 >-> base_lit.
-Coercion LitInt32 : u32 >-> base_lit.
-Coercion LitInt16 : w16 >-> base_lit.
-Coercion LitByte : u8 >-> base_lit.
-Coercion LitProphecy : proph_id >-> base_lit.
-Notation "'str' s" := (LitString (s : byte_string)) (at level 30, format "'str'  s") : val_scope.
-
-Definition b2val {ext: ffi_syntax}: u8 -> val := λ (b:u8), LitV (LitByte b).
-Global Instance b2val_inj {ext: ffi_syntax} : Inj eq eq b2val.
-Proof.
-  intros b1 b2 Heq.
-  inversion Heq; auto.
-Qed.
 
 Coercion App : expr >-> Funclass.
 
@@ -369,19 +333,6 @@ Notation Lam x e := (Rec BAnon x e) (only parsing).
 Notation Let x e1 e2 := (App (Lam x e2) e1) (only parsing).
 Notation Seq e1 e2 := (Let BAnon e1 e2) (only parsing).
 Notation LamV x e := (RecV BAnon x e) (only parsing).
-Notation Match e0 x1 e1 x2 e2 := (Case e0 (Lam x1 e1) (Lam x2 e2)) (only parsing).
-Notation Alloc e := (AllocN (Val $ LitV $ LitInt (W64 1)) e).
-(** Compare-and-set (CAS) returns just a boolean indicating success or failure. *)
-Notation CAS l e1 e2 := (Snd (CmpXchg l e1 e2)) (only parsing).
-
-(* Skip should be atomic, we sometimes open invariants around
-   it. Hence, we need to explicitly use LamV instead of e.g., Seq. *)
-Notation Skip := (App (Val $ LamV BAnon (Val $ LitV LitUnit)) (Val $ LitV LitUnit)).
-Definition Linearize {ext:ffi_syntax}: expr := Skip.
-
-(* No scope for the values, does not conflict and scope is often not inferred
-properly. *)
-Notation "# l" := (LitV l%Z%V%stdpp) (at level 8, format "# l").
 
 (** Syntax inspired by Coq/Ocaml. Constructions with higher precedence come
     first. *)
@@ -410,52 +361,9 @@ Moreover, if the branches do not fit on a single line, it will be printed as:
     even more stuff bla bla bla bla bla bla bla bla
   end
 *)
-Notation "'match:' e0 'with' 'InjL' x1 => e1 | 'InjR' x2 => e2 'end'" :=
-  (Match e0 x1%binder e1 x2%binder e2)
-  (e0, x1, e1, x2, e2 at level 200,
-   format "'[hv' 'match:'  e0  'with'  '/  ' '[' 'InjL'  x1  =>  '/  ' e1 ']'  '/' '[' |  'InjR'  x2  =>  '/  ' e2 ']'  '/' 'end' ']'") : expr_scope.
-Notation "'match:' e0 'with' 'InjR' x1 => e1 | 'InjL' x2 => e2 'end'" :=
-  (Match e0 x2%binder e2 x1%binder e1)
-  (e0, x1, e1, x2, e2 at level 200, only parsing) : expr_scope.
 
-Notation "()" := LitUnit : val_scope.
 Notation "! e" := (Load e%E) (at level 9, right associativity) : expr_scope.
-Notation "'ref' e" := (Alloc e%E) (at level 10) : expr_scope.
-Notation "- e" := (UnOp MinusUnOp e%E) : expr_scope.
-Notation "'u_to_w64' e" := (UnOp UToW64Op e%E) (at level 10) : expr_scope.
-Notation "'u_to_w32' e" := (UnOp UToW32Op e%E) (at level 10) : expr_scope.
-Notation "'u_to_w16' e" := (UnOp UToW16Op e%E) (at level 10) : expr_scope.
-Notation "'u_to_w8' e" := (UnOp UToW8Op e%E) (at level 10) : expr_scope.
-Notation "'s_to_w64' e" := (UnOp SToW64Op e%E) (at level 10) : expr_scope.
-Notation "'s_to_w32' e" := (UnOp SToW32Op e%E) (at level 10) : expr_scope.
-Notation "'s_to_w16' e" := (UnOp SToW16Op e%E) (at level 10) : expr_scope.
-Notation "'s_to_w8' e" := (UnOp SToW8Op e%E) (at level 10) : expr_scope.
-Notation "'to_u64' e" := (UnOp UToW64Op e%E) (at level 10, only parsing) : expr_scope. (* backwards compatibility *)
-Notation "'to_u32' e" := (UnOp UToW32Op e%E) (at level 10, only parsing) : expr_scope. (* backwards compatibility *)
-Notation "'to_u16' e" := (UnOp UToW16Op e%E) (at level 10, only parsing) : expr_scope. (* backwards compatibility *)
-Notation "'to_u8' e" := (UnOp UToW8Op e%E) (at level 10, only parsing) : expr_scope. (* backwards compatibility *)
-Notation "'to_string' e" := (UnOp ToStringOp e%E) (at level 10) : expr_scope.
-Notation "'StringLength' e" := (UnOp StringLenOp e%E) (at level 10) : expr_scope.
-Notation "'IsNoStringOverflow' e" := (UnOp IsNoStringOverflowOp e%E) (at level 10) : expr_scope.
 
-Notation "'StringGet'" := (BinOp StringGetOp) (at level 10) : expr_scope.
-Notation "e1 + e2" := (BinOp PlusOp e1%E e2%E) : expr_scope.
-Notation "e1 +ₗ e2" := (BinOp (OffsetOp 1) e1%E e2%E) : expr_scope.
-Notation "e1 - e2" := (BinOp MinusOp e1%E e2%E) : expr_scope.
-Notation "e1 * e2" := (BinOp MultOp e1%E e2%E) : expr_scope.
-Notation "e1 `or` e2" := (BinOp OrOp e1%E e2%E) (at level 40) : expr_scope.
-Notation "e1 `and` e2" := (BinOp AndOp e1%E e2%E) (at level 40) : expr_scope.
-Notation "e1 `xor` e2" := (BinOp XorOp e1%E e2%E) (at level 40) : expr_scope.
-Notation "e1 `quot` e2" := (BinOp QuotOp e1%E e2%E) : expr_scope.
-Notation "e1 `quots` e2" := (BinOp QuotSignedOp e1%E e2%E) (at level 35) : expr_scope.
-Notation "e1 `rem` e2" := (BinOp RemOp e1%E e2%E) : expr_scope.
-Notation "e1 `rems` e2" := (BinOp RemSignedOp e1%E e2%E) (at level 35) : expr_scope.
-Notation "e1 ≪ e2" := (BinOp ShiftLOp e1%E e2%E) : expr_scope.
-Notation "e1 ≫ e2" := (BinOp ShiftROp e1%E e2%E) : expr_scope.
-(* models Go's &^ operator *)
-Notation "e1 `and_not` e2" := (BinOp AndOp e1%E (UnOp NegOp e2%E)) (at level 40, only parsing) : expr_scope.
-
-Notation "~ e" := (UnOp NegOp e%E) (at level 75, right associativity) : expr_scope.
 Definition Store {ext:ffi_syntax} : val :=
   LamV "l" (Lam "v" (Seq
                      (PrepareWrite (Var "l"))
@@ -557,25 +465,6 @@ Notation "e1 ;; e2" := (Lam BAnon e2%E e1%E)
   (at level 100, e2 at level 200,
    format "'[' '[hv' '[' e1 ']' ;;  ']' '/' e2 ']'") : expr_scope.
 
-(* Shortcircuit Boolean connectives *)
-Notation "e1 && e2" :=
-  (If e1%E e2%E (LitV (LitBool false))) (only parsing) : expr_scope.
-Notation "e1 || e2" :=
-  (If e1%E (LitV (LitBool true)) e2%E) (only parsing) : expr_scope.
-
-(** Notations for option *)
-Notation NONE := (InjL (LitV LitUnit)) (only parsing).
-Notation NONEV := (InjLV (LitV LitUnit)) (only parsing).
-Notation SOME x := (InjR x) (only parsing).
-Notation SOMEV x := (InjRV x) (only parsing).
-
-Notation "'match:' e0 'with' 'NONE' => e1 | 'SOME' x => e2 'end'" :=
-  (Match e0 BAnon e1 x%binder e2)
-  (e0, e1, x, e2 at level 200, only parsing) : expr_scope.
-Notation "'match:' e0 'with' 'SOME' x => e2 | 'NONE' => e1 'end'" :=
-  (Match e0 BAnon e1 x%binder e2)
-  (e0, e1, x, e2 at level 200, only parsing) : expr_scope.
-
 (*
 Notation ResolveProph e1 e2 := (Resolve Skip e1 e2) (only parsing).
 Notation "'resolve_proph:' p 'to:' v" := (ResolveProph p v) (at level 100) : expr_scope.
@@ -599,7 +488,12 @@ End func.
 Class GoGlobalContext {ext : ffi_syntax} : Type :=
   {
     into_val : ∀ {V : Type} (v : V), val;
+    #[global] into_val_inj_loc :: Inj eq eq (into_val (V:=loc));
+    #[global] into_val_inj_bool ::  Inj eq eq (into_val (V:=bool));
+    #[global] into_val_inj_proph_id ::  Inj eq eq (into_val (V:=proph_id));
   }.
+Global Notation "# x" := (into_val x%go) (at level 8).
+Global Notation "#" := into_val (at level 0).
 
 (** [GoLocalContext] contains several low-level Go functions for typed memory access,
     map updates, etc. *)
@@ -644,16 +538,6 @@ Section external.
 (* these are codes for external operations (which all take a single val as an
    argument and evaluate to a value) and data for external values *)
 Context {ext : ffi_syntax}.
-
-(* XXX: to avoid splitting things into heap cells, can wrap it in e.g. an InjLV.
-   This is how lists can avoid getting split into different heap cells when [ref]'d. *)
-Fixpoint flatten_struct (v: val) : list val :=
-  match v with
-  | PairV v1 v2 => flatten_struct v1 ++ flatten_struct v2
-  | LitV LitUnit => []
-  | _ => [v]
-  end.
-
 Context {ffi : ffi_model}.
 
 Inductive naMode : Set :=
@@ -664,27 +548,6 @@ Notation nonAtomic T := (naMode * T)%type.
 
 (* TODO: Free should really be called something else - quiescent? just value?  *)
 Definition Free {T} (v:T): nonAtomic T := (Reading 0, v).
-
-Inductive event :=
-  | In_ev (sel v:base_lit)
-  | Out_ev (v:base_lit)
-  | Crash_ev
-.
-
-(* a trace is a list of events, stored in reverse order *)
-Definition Trace := list event.
-
-Definition add_event (ev: event) (ts: Trace) : Trace := cons ev ts.
-
-Definition add_crash (ts: Trace) : Trace :=
-  match ts with
-  | Crash_ev::ts' => ts
-  | _ => add_event Crash_ev ts
-  end.
-
-Definition Oracle := Trace -> forall (sel:u64), u64.
-
-Instance Oracle_Inhabited: Inhabited Oracle := populate (fun _ _ => word.of_Z 0).
 
 Class ZeroVal V :=
   {
@@ -745,10 +608,8 @@ Notation "e1 && e2" :=
 Notation "e1 || e2" :=
   (If e1%E #true e2%E) (only parsing) : expr_scope.
 
-Local Notation "# x" := (into_val x%go).
-Local Notation "#" := into_val (at level 0).
-
-Definition is_go_step `{!GoGlobalContext} `{!GoLocalContext}
+Context {go_gctx : GoGlobalContext}.
+Definition is_go_step `{!GoLocalContext}
   (op : go_instruction) (arg : val) (e' : expr) (s s' : gmap go_string bool) : Prop :=
   match op with
   | PackageInitCheck p => arg = #() ∧ e' = #(default false (s !! p)) ∧ s' = s
@@ -767,18 +628,15 @@ Record state : Type := {
   heap : gmap loc (nonAtomic val);
   go_state : GoState;
   world : ffi_state;
-  trace : Trace;
-  oracle : Oracle;
 }.
 Record global_state : Type := {
   global_world: ffi_global_state;
   used_proph_id: gset proph_id;
-  go_gctx : GoGlobalContext;
 }.
 
 Global Instance eta_go_state : Settable _ := settable! Build_GoState <go_lctx; package_state>.
-Global Instance eta_state : Settable _ := settable! Build_state <heap; go_state; world; trace; oracle>.
-Global Instance eta_global_state : Settable _ := settable! Build_global_state <global_world; used_proph_id; go_gctx>.
+Global Instance eta_state : Settable _ := settable! Build_state <heap; go_state; world >.
+Global Instance eta_global_state : Settable _ := settable! Build_global_state <global_world; used_proph_id>.
 
 (* Note that ffi_step takes a val, which is itself parameterized by the
 external type, so the semantics of external operations depend on a definition of
@@ -806,7 +664,8 @@ Inductive goose_crash : state -> state -> Prop :=
   | GooseCrash σ w w' go_state' :
      w = σ.(world) ->
      ffi_crash_step w w' ->
-     goose_crash σ (set go_state (fun _ => go_state') (set trace add_crash (set world (fun _ => w') (set heap (fun _ => ∅) σ))))
+     goose_crash σ
+       (set go_state (fun _ => go_state') (set world (fun _ => w') (set heap (fun _ => ∅) σ)))
 .
 
 
@@ -866,17 +725,15 @@ Global Instance comm_clause_inhabited : Inhabited comm_clause := populate (CommC
 
 Global Instance func_t_inhabited : Inhabited func.t :=
   populate (func.mk inhabitant inhabitant inhabitant).
-Global Instance GoGlobalContext_inhabited : Inhabited GoGlobalContext :=
-  populate {| into_val := inhabitant |}.
 Global Instance GoLocalContext_inhabited : Inhabited GoLocalContext :=
   populate {| is_go_step_pure := inhabitant; |}.
 Global Instance GoState_inhabited : Inhabited GoState :=
   populate {| go_lctx := inhabitant; package_state := inhabitant |}.
 
 Global Instance state_inhabited : Inhabited state :=
-  populate {| heap := inhabitant; go_state := inhabitant; world := inhabitant; trace := inhabitant; oracle := inhabitant; |}.
+  populate {| heap := inhabitant; go_state := inhabitant; world := inhabitant; |}.
 Global Instance global_state_inhabited : Inhabited global_state :=
-  populate {| used_proph_id := inhabitant; global_world := inhabitant; go_gctx := inhabitant |}.
+  populate {| used_proph_id := inhabitant; global_world := inhabitant |}.
 
 Canonical Structure stateO := leibnizO state.
 Canonical Structure locO := leibnizO loc.
@@ -891,17 +748,11 @@ Canonical Structure u8O := leibnizO u8.
 Inductive ectx_item :=
   | AppLCtx (v2 : val)
   | AppRCtx (e1 : expr)
-  | UnOpCtx (op : un_op)
-  | BinOpLCtx (op : bin_op) (e2 : expr)
-  | BinOpRCtx (op : bin_op) (v1 : val)
   | IfCtx (e1 e2 : expr)
   | PairLCtx (e2 : expr)
   | PairRCtx (v1 : val)
   | FstCtx
   | SndCtx
-  | InjLCtx
-  | InjRCtx
-  | CaseCtx (e1 : expr) (e2 : expr)
   | Primitive1Ctx  (op: prim_op args1)
   | Primitive2LCtx (op: prim_op args2) (e2 : expr)
   | Primitive2RCtx (op: prim_op args2) (v1 : val)
@@ -909,38 +760,24 @@ Inductive ectx_item :=
   | Primitive3MCtx (op: prim_op args3) (v0 : val) (e2 : expr)
   | Primitive3RCtx (op: prim_op args3) (v0 : val) (v1 : val) *)
   | ExternalOpCtx (op : ffi_opcode)
-  | CmpXchgLCtx (e1 : expr) (e2 : expr)
-  | CmpXchgMCtx (v1 : val) (e2 : expr)
-  | CmpXchgRCtx (v1 : val) (v2 : val)
   | ResolveProphLCtx (v2 : val)
-  | ResolveProphRCtx (e1 : expr)
-  | AtomicallyCtx (e0 : expr).
+  | ResolveProphRCtx (e1 : expr).
 
 Definition fill_item (Ki : ectx_item) (e : expr) : expr :=
   match Ki with
   | AppLCtx v2 => App e (of_val v2)
   | AppRCtx e1 => App e1 e
-  | UnOpCtx op => UnOp op e
-  | BinOpLCtx op e2 => BinOp op e e2
-  | BinOpRCtx op v1 => BinOp op (Val v1) e
   | IfCtx e1 e2 => If e e1 e2
   | PairLCtx e2 => Pair e e2
   | PairRCtx v1 => Pair (Val v1) e
   | FstCtx => Fst e
   | SndCtx => Snd e
-  | InjLCtx => InjL e
-  | InjRCtx => InjR e
-  | CaseCtx e1 e2 => Case e e1 e2
   | Primitive1Ctx op => Primitive1 op e
   | Primitive2LCtx op e2 => Primitive2 op e e2
   | Primitive2RCtx op v1 => Primitive2 op (Val v1) e
   | ExternalOpCtx op => ExternalOp op e
-  | CmpXchgLCtx e1 e2 => CmpXchg e e1 e2
-  | CmpXchgMCtx v0 e2 => CmpXchg (Val v0) e e2
-  | CmpXchgRCtx v0 v1 => CmpXchg (Val v0) (Val v1) e
   | ResolveProphLCtx v2 => ResolveProph e (Val v2)
   | ResolveProphRCtx e1 => ResolveProph e1 e
-  | AtomicallyCtx e1 => Atomically e e1
   end.
 
 (** Substitution *)
@@ -951,23 +788,16 @@ Fixpoint subst (x : string) (v : val) (e : expr)  : expr :=
   | Rec f y e =>
      Rec f y $ if decide (BNamed x ≠ f ∧ BNamed x ≠ y) then subst x v e else e
   | App e1 e2 => App (subst x v e1) (subst x v e2)
-  | UnOp op e => UnOp op (subst x v e)
-  | BinOp op e1 e2 => BinOp op (subst x v e1) (subst x v e2)
   | If e0 e1 e2 => If (subst x v e0) (subst x v e1) (subst x v e2)
   | Pair e1 e2 => Pair (subst x v e1) (subst x v e2)
   | Fst e => Fst (subst x v e)
   | Snd e => Snd (subst x v e)
-  | InjL e => InjL (subst x v e)
-  | InjR e => InjR (subst x v e)
-  | Case e0 e1 e2 => Case (subst x v e0) (subst x v e1) (subst x v e2)
   | Fork e => Fork (subst x v e)
-  | Atomically el e => Atomically (subst x v el) (subst x v e)
   | Primitive0 op => Primitive0 op
   | Primitive1 op e => Primitive1 op (subst x v e)
   | Primitive2 op e1 e2 => Primitive2 op (subst x v e1) (subst x v e2)
   (* | Primitive3 op e1 e2 e3 => Primitive3 op (subst x v e1) (subst x v e2) (subst x v e3) *)
   | ExternalOp op e => ExternalOp op (subst x v e)
-  | CmpXchg e0 e1 e2 => CmpXchg (subst x v e0) (subst x v e1) (subst x v e2)
   | NewProph => NewProph
   | ResolveProph e1 e2 => ResolveProph (subst x v e1) (subst x v e2)
   | LiteralValue l => LiteralValue ((subst_keyed_element x v) <$> l)
@@ -1004,123 +834,6 @@ Definition subst' (mx : binder) (v : val) : expr → expr :=
   match mx with BNamed x => subst x v | BAnon => id end.
 
 (** The stepping relation *)
-Definition un_op_eval (op : un_op) (v : val) : option val :=
-  match op, v with
-  | NegOp, LitV (LitBool b) => Some $ LitV $ LitBool (negb b)
-  | NegOp, LitV (LitInt n) => Some $ LitV $ LitInt (word.not n)
-  | NegOp, LitV (LitInt32 n) => Some $ LitV $ LitInt32 (word.not n)
-  | NegOp, LitV (LitInt16 n) => Some $ LitV $ LitInt16 (word.not n)
-  | MinusUnOp, LitV (LitByte n) => Some $ LitV $ LitByte (word.opp n)
-  | MinusUnOp, LitV (LitInt n) => Some $ LitV $ LitInt (word.opp n)
-  | MinusUnOp, LitV (LitInt32 n) => Some $ LitV $ LitInt32 (word.opp n)
-  | MinusUnOp, LitV (LitInt16 n) => Some $ LitV $ LitInt16 (word.opp n)
-  | NegOp, LitV (LitByte n) => Some $ LitV $ LitByte (word.not n)
-  | UToW64Op, LitV (LitInt v)   => Some $ LitV $ LitInt (W64 (uint.Z v))
-  | UToW64Op, LitV (LitInt32 v) => Some $ LitV $ LitInt (W64 (uint.Z v))
-  | UToW64Op, LitV (LitInt16 v) => Some $ LitV $ LitInt (W64 (uint.Z v))
-  | UToW64Op, LitV (LitByte v)  => Some $ LitV $ LitInt (W64 (uint.Z v))
-  | UToW32Op, LitV (LitInt v)   => Some $ LitV $ LitInt32 (W32 (uint.Z v))
-  | UToW32Op, LitV (LitInt32 v) => Some $ LitV $ LitInt32 (W32 (uint.Z v))
-  | UToW32Op, LitV (LitInt16 v) => Some $ LitV $ LitInt32 (W32 (uint.Z v))
-  | UToW32Op, LitV (LitByte v)  => Some $ LitV $ LitInt32 (W32 (uint.Z v))
-  | UToW16Op, LitV (LitInt v)   => Some $ LitV $ LitInt16 (W16 (uint.Z v))
-  | UToW16Op, LitV (LitInt32 v) => Some $ LitV $ LitInt16 (W16 (uint.Z v))
-  | UToW16Op, LitV (LitInt16 v) => Some $ LitV $ LitInt16 (W16 (uint.Z v))
-  | UToW16Op, LitV (LitByte v)  => Some $ LitV $ LitInt16 (W16 (uint.Z v))
-  | UToW8Op, LitV (LitInt v)    => Some $ LitV $ LitByte (W8 (uint.Z v))
-  | UToW8Op, LitV (LitInt32 v)  => Some $ LitV $ LitByte (W8 (uint.Z v))
-  | UToW8Op, LitV (LitInt16 v)  => Some $ LitV $ LitByte (W8 (uint.Z v))
-  | UToW8Op, LitV (LitByte v)   => Some $ LitV $ LitByte (W8 (uint.Z v))
-  | SToW64Op, LitV (LitInt v)   => Some $ LitV $ LitInt (W64 (sint.Z v))
-  | SToW64Op, LitV (LitInt32 v) => Some $ LitV $ LitInt (W64 (sint.Z v))
-  | SToW64Op, LitV (LitInt16 v) => Some $ LitV $ LitInt (W64 (sint.Z v))
-  | SToW64Op, LitV (LitByte v)  => Some $ LitV $ LitInt (W64 (sint.Z v))
-  | SToW32Op, LitV (LitInt v)   => Some $ LitV $ LitInt32 (W32 (sint.Z v))
-  | SToW32Op, LitV (LitInt32 v) => Some $ LitV $ LitInt32 (W32 (sint.Z v))
-  | SToW32Op, LitV (LitInt16 v) => Some $ LitV $ LitInt32 (W32 (sint.Z v))
-  | SToW32Op, LitV (LitByte v)  => Some $ LitV $ LitInt32 (W32 (sint.Z v))
-  | SToW16Op, LitV (LitInt v)   => Some $ LitV $ LitInt16 (W16 (sint.Z v))
-  | SToW16Op, LitV (LitInt32 v) => Some $ LitV $ LitInt16 (W16 (sint.Z v))
-  | SToW16Op, LitV (LitInt16 v) => Some $ LitV $ LitInt16 (W16 (sint.Z v))
-  | SToW16Op, LitV (LitByte v)  => Some $ LitV $ LitInt16 (W16 (sint.Z v))
-  | SToW8Op, LitV (LitInt v)    => Some $ LitV $ LitByte (W8 (sint.Z v))
-  | SToW8Op, LitV (LitInt32 v)  => Some $ LitV $ LitByte (W8 (sint.Z v))
-  | SToW8Op, LitV (LitInt16 v)  => Some $ LitV $ LitByte (W8 (sint.Z v))
-  | SToW8Op, LitV (LitByte v)   => Some $ LitV $ LitByte (W8 (sint.Z v))
-  | ToStringOp, LitV (LitByte v) => Some $ LitV $ LitString [v]
-  | StringLenOp, LitV (LitString v) => Some $ LitV $ LitInt (W64 (Z.of_nat (length v)))
-  | IsNoStringOverflowOp, LitV (LitString v) => Some $ LitV $ LitBool (bool_decide (Z.of_nat (length v) < 2^63))
-  | _, _ => None
-  end.
-
-Definition bin_op_eval_word (op : bin_op) {width} {word: Interface.word width} (n1 n2 : word) : option word :=
-  match op with
-  | PlusOp => Some $ word.add (word:=word) n1 n2
-  | MinusOp => Some $ word.sub (word:=word) n1 n2
-  | MultOp => Some $ (word.mul (word:=word) n1 n2)
-  | QuotOp => Some $ (word.divu (word:=word) n1 n2)
-  | QuotSignedOp => Some $ (word.divs (word:=word) n1 n2)
-  | RemOp => Some $ (word.modu (word:=word) n1 n2)
-  | RemSignedOp => Some $ (word.mods (word:=word) n1 n2)
-  | AndOp => Some $ (word.and (word:=word) n1 n2)
-  | OrOp => Some $ (word.or (word:=word) n1 n2)
-  | XorOp => Some $ (word.xor (word:=word) n1 n2)
-  | ShiftLOp => Some $ (word.slu (word:=word) n1 n2)
-  | ShiftROp => Some $ (word.sru (word:=word) n1 n2)
-  | _ => None
-  end.
-
-Definition bin_op_eval_shift (op : bin_op) {width} {word: Interface.word width} (n1 n2 : word) : option word :=
-  if decide (op = ShiftLOp ∨ op = ShiftROp) then
-    bin_op_eval_word op n1 n2
-  else None.
-
-Definition bin_op_eval_compare (op : bin_op) {width} {word: Interface.word width} (n1 n2 : word) : option bool :=
-  match op with
-  | LeOp => Some $ bool_decide (word.unsigned n1 <= word.unsigned n2)
-  | LtOp => Some $ bool_decide (word.unsigned n1 < word.unsigned n2)
-  | EqOp => Some $ bool_decide (word.unsigned n1 = word.unsigned n2)
-  | _ => None
-  end.
-
-Definition bin_op_eval_bool (op : bin_op) (b1 b2 : bool) : option bool :=
-  match op with
-  | PlusOp | MinusOp | MultOp | QuotOp | RemOp => None (* Arithmetic *)
-  | AndOp => Some (b1 && b2)
-  | OrOp => Some (b1 || b2)
-  | XorOp => Some (xorb b1 b2)
-  | ShiftLOp | ShiftROp => None (* Shifts *)
-  | LeOp | LtOp => None (* InEquality *)
-  | EqOp => Some (bool_decide (b1 = b2))
-  | OffsetOp _ => None (* Pointer arithmetic *)
-  | _ => None
-  end.
-
-Definition bin_op_eval_string (op : bin_op) (s1 s2 : byte_string) : option byte_string :=
-  match op with
-  | PlusOp => Some $ (s1 ++ s2)
-  | _ => None
-  end.
-
-Definition bin_op_eval_string_word (op : bin_op) (s1 : byte_string) {width} {word: Interface.word width} (w2 : word): option w8 :=
-  match op with
-  | StringGetOp => (s1 !! (uint.nat w2))
-  | _ => None
-  end.
-
-(* exclude some comparisons *)
-Fixpoint is_comparable v :=
-  match v with
-  | RecV _ _ _ | ExtV _ => False
-  | PairV v1 v2 => is_comparable v1 ∧ is_comparable v2
-  | InjLV v => is_comparable v
-  | InjRV v => is_comparable v
-  | _ => True
-  end.
-Global Instance is_comparable_decide v : Decision (is_comparable v).
-Proof.
-  induction v; simpl; auto; solve_decision.
-Defined.
 
 Section instances.
 Inductive tree (T : Type) : Type :=
@@ -1189,21 +902,14 @@ Fixpoint enc_expr (v : expr) : tree leaf_type :=
   | Var arg1 => Node "Var" [Leaf $ StringLeaf arg1]
   | Rec arg1 arg2 arg3 => Node "Rec" [Leaf $ BinderLeaf arg1; Leaf $ BinderLeaf arg2; enc_expr arg3]
   | App arg1 arg2 => Node "App" [enc_expr arg1; enc_expr arg2]
-  | UnOp arg1 arg2 => Node "UnOp" [Leaf $ UnOpLeaf arg1; enc_expr arg2]
-  | BinOp arg1 arg2 arg3 => Node "BinOp" [Leaf $ BinOpLeaf arg1; enc_expr arg2; enc_expr arg3]
   | If arg1 arg2 arg3 => Node "If" [enc_expr arg1; enc_expr arg2; enc_expr arg3]
   | Pair arg1 arg2 => Node "Pair" [enc_expr arg1; enc_expr arg2]
   | Fst arg1 => Node "Fst" [enc_expr arg1]
   | Snd arg1 => Node "Snd" [enc_expr arg1]
-  | InjL arg1 => Node "InjL" [enc_expr arg1]
-  | InjR arg1 => Node "InjR" [enc_expr arg1]
-  | Case arg1 arg2 arg3 => Node "Case" [enc_expr arg1; enc_expr arg2; enc_expr arg3]
   | Fork arg1 => Node "Fork" [enc_expr arg1]
-  | Atomically arg1 arg2 => Node "Atomically" [enc_expr arg1; enc_expr arg2]
   | Primitive0 arg1 => Node "Primitive0" [Leaf $ PrimOpArgs0Leaf arg1]
   | Primitive1 arg1 arg2 => Node "Primitive1" [Leaf $ PrimOpArgs1Leaf arg1; enc_expr arg2]
   | Primitive2 arg1 arg2 arg3 => Node "Primitive2" [Leaf $ PrimOpArgs2Leaf arg1; enc_expr arg2; enc_expr arg3]
-  | CmpXchg arg1 arg2 arg3 => Node "CmpXchg" [enc_expr arg1; enc_expr arg2; enc_expr arg3]
   | ExternalOp arg1 arg2 => Node "ExternalOp" [Leaf $ FfiOpcodeLeaf arg1; enc_expr arg2]
   | NewProph  => Node "NewProph" []
   | ResolveProph arg1 arg2 => Node "ResolveProph" [enc_expr arg1; enc_expr arg2]
@@ -1279,25 +985,16 @@ Fixpoint dec_expr (v : tree leaf_type) : expr :=
   | Node "Rec" [Leaf (BinderLeaf arg1); Leaf (BinderLeaf arg2); arg3] =>
        Rec arg1 arg2 (dec_expr arg3)
   | Node "App" [arg1; arg2] => App (dec_expr arg1) (dec_expr arg2)
-  | Node "UnOp" [Leaf (UnOpLeaf arg1); arg2] => UnOp arg1 (dec_expr arg2)
-  | Node "BinOp" [Leaf (BinOpLeaf arg1); arg2; arg3] =>
-      BinOp arg1 (dec_expr arg2) (dec_expr arg3)
   | Node "If" [arg1; arg2; arg3] => If (dec_expr arg1) (dec_expr arg2) (dec_expr arg3)
   | Node "Pair" [arg1; arg2] => Pair (dec_expr arg1) (dec_expr arg2)
   | Node "Fst" [arg1] => Fst (dec_expr arg1)
   | Node "Snd" [arg1] => Snd (dec_expr arg1)
-  | Node "InjL" [arg1] => InjL (dec_expr arg1)
-  | Node "InjR" [arg1] => InjR (dec_expr arg1)
-  | Node "Case" [arg1; arg2; arg3] => Case (dec_expr arg1) (dec_expr arg2) (dec_expr arg3)
   | Node "Fork" [arg1] => Fork (dec_expr arg1)
-  | Node "Atomically" [arg1; arg2] => Atomically (dec_expr arg1) (dec_expr arg2)
   | Node "Primitive0" [Leaf (PrimOpArgs0Leaf arg1)] => Primitive0 arg1
   | Node "Primitive1" [Leaf (PrimOpArgs1Leaf arg1); arg2] =>
        Primitive1 arg1 (dec_expr arg2)
   | Node "Primitive2" [Leaf (PrimOpArgs2Leaf arg1); arg2; arg3] =>
        Primitive2 arg1 (dec_expr arg2) (dec_expr arg3)
-  | Node "CmpXchg" [arg1; arg2; arg3] =>
-       CmpXchg (dec_expr arg1) (dec_expr arg2) (dec_expr arg3)
   | Node "ExternalOp" [Leaf (FfiOpcodeLeaf arg1); arg2] =>
        ExternalOp arg1 (dec_expr arg2)
   | Node "NewProph" [] => NewProph
@@ -1474,84 +1171,9 @@ Qed.
 
 End instances.
 
-Definition bin_op_eval_eq (v1 v2 : val) : option base_lit :=
-  if decide (is_comparable v1 ∧ is_comparable v2) then
-    Some $ LitBool $ bool_decide (v1 = v2)
-  else None.
-
-Definition bin_op_eval (op : bin_op) (v1 v2 : val) : option val :=
-  if decide (op = EqOp) then LitV <$> bin_op_eval_eq v1 v2
-  else
-    match v1, v2 with
-    | LitV (LitInt n1), LitV (LitInt n2) =>
-      LitV <$> ((LitInt <$> bin_op_eval_word op n1 n2)
-                  ∪ (LitBool <$> bin_op_eval_compare op n1 n2))
-    | LitV (LitInt32 n1), LitV (LitInt32 n2) =>
-      LitV <$> ((LitInt32 <$> bin_op_eval_word op n1 n2)
-                  ∪ (LitBool <$> bin_op_eval_compare op n1 n2))
-    | LitV (LitInt16 n1), LitV (LitInt16 n2) =>
-      LitV <$> ((LitInt16 <$> bin_op_eval_word op n1 n2)
-                  ∪ (LitBool <$> bin_op_eval_compare op n1 n2))
-    | LitV (LitByte n1), LitV (LitByte n2) =>
-      LitV <$> ((LitByte <$> bin_op_eval_word op n1 n2)
-                  ∪ (LitBool <$> bin_op_eval_compare op n1 n2))
-
-    (* Shifts do not require matching bit width *)
-    | LitV (LitByte n1), LitV (LitInt n2) =>
-      LitV <$> (LitByte <$> bin_op_eval_shift op n1 (W8 (uint.Z n2)))
-    | LitV (LitByte n1), LitV (LitInt32 n2) =>
-      LitV <$> (LitByte <$> bin_op_eval_shift op n1 (W8 (uint.Z n2)))
-    | LitV (LitByte n1), LitV (LitInt16 n2) =>
-      LitV <$> (LitByte <$> bin_op_eval_shift op n1 (W8 (uint.Z n2)))
-    | LitV (LitInt16 n1), LitV (LitInt n2) =>
-      LitV <$> (LitInt16 <$> bin_op_eval_shift op n1 (W16 (uint.Z n2)))
-    | LitV (LitInt16 n1), LitV (LitInt32 n2) =>
-      LitV <$> (LitInt16 <$> bin_op_eval_shift op n1 (W16 (uint.Z n2)))
-    | LitV (LitInt16 n1), LitV (LitByte n2) =>
-      LitV <$> (LitInt16 <$> bin_op_eval_shift op n1 (W16 (uint.Z n2)))
-    | LitV (LitInt32 n1), LitV (LitInt n2) =>
-      LitV <$> (LitInt32 <$> bin_op_eval_shift op n1 (W32 (uint.Z n2)))
-    | LitV (LitInt32 n1), LitV (LitInt16 n2) =>
-      LitV <$> (LitInt32 <$> bin_op_eval_shift op n1 (W32 (uint.Z n2)))
-    | LitV (LitInt32 n1), LitV (LitByte n2) =>
-      LitV <$> (LitInt32 <$> bin_op_eval_shift op n1 (W32 (uint.Z n2)))
-    | LitV (LitInt n1), LitV (LitByte n2) =>
-      LitV <$> (LitInt <$> bin_op_eval_shift op n1 (W64 (uint.Z n2)))
-    | LitV (LitInt n1), LitV (LitInt16 n2) =>
-      LitV <$> (LitInt <$> bin_op_eval_shift op n1 (W64 (uint.Z n2)))
-    | LitV (LitInt n1), LitV (LitInt32 n2) =>
-      LitV <$> (LitInt <$> bin_op_eval_shift op n1 (W64 (uint.Z n2)))
-
-    | LitV (LitBool b1), LitV (LitBool b2) => LitV <$> (LitBool <$> bin_op_eval_bool op b1 b2)
-    | LitV (LitString s1), LitV (LitString s2) => LitV <$> (LitString <$> bin_op_eval_string op s1 s2)
-    | LitV (LitLoc l), LitV (LitInt off) => match op with
-                                           | OffsetOp k =>
-                                             Some $ LitV $ LitLoc (l +ₗ k * (uint.Z (off: u64)))
-                                           | _ => None
-                                           end
-    | LitV (LitString s1), LitV (LitByte n) => LitV <$> (LitByte <$> bin_op_eval_string_word op s1 n)
-    | LitV (LitString s1), LitV (LitInt16 n) => LitV <$> (LitByte <$> bin_op_eval_string_word op s1 n)
-    | LitV (LitString s1), LitV (LitInt32 n) => LitV <$> (LitByte <$> bin_op_eval_string_word op s1 n)
-    | LitV (LitString s1), LitV (LitInt n) => LitV <$> (LitByte <$> bin_op_eval_string_word op s1 n)
-    | _, _ => None
-    end.
-
 (* [h] is added on the right here to make [state_init_heap_singleton] true. *)
-Definition state_insert_list (l: loc) (vs: list val) (σ: state): state :=
-  set heap (λ h, heap_array l (fmap Free vs) ∪ h) σ.
-
-Definition concat_replicate {A} (n: nat) (l: list A): list A :=
-  concat (replicate n l).
-
-Definition state_init_heap (l : loc) (n : Z) (v : val) (σ : state) : state :=
-  state_insert_list l (concat_replicate (Z.to_nat n) (flatten_struct v)) σ.
-
-Lemma state_init_heap_singleton l v σ :
-  state_init_heap l 1 v σ = state_insert_list l (flatten_struct v) σ.
-Proof.
-  destruct σ as [h p]. rewrite /state_init_heap /concat_replicate /state_insert_list /set /=. f_equal.
-  rewrite right_id. done.
-Qed.
+Definition state_init_heap (l : loc) (v : val) (σ : state) : state :=
+  set heap (λ h, {[ l := Free v ]} ∪ h) σ.
 
 Definition is_Free {A} (mna: option (nonAtomic A)) := exists x, mna = Some (Free x).
 Global Instance is_Free_dec A (x: option (nonAtomic A)) : Decision (is_Free x).
@@ -1616,32 +1238,18 @@ Qed.
 Theorem isFresh_not_null σ l :
   isFresh σ l -> l ≠ null.
 Proof.
-  intros Hbound **.
-  rewrite -(loc_add_0 l).
-  eapply Hbound.
-Qed.
-
-Theorem isFresh_offset0 σ l :
-  isFresh σ l -> addr_offset l = 0.
-Proof.
-  intros Hbound. destruct Hbound as (?&?); eauto.
-Qed.
-
-Theorem isFresh_base σ l :
-  isFresh σ l -> addr_base l = l.
-Proof.
-  intros Hbound **. eapply addr_offset_0_is_base, isFresh_offset0; eauto.
+  intros Hbound **. rewrite -(loc_add_0 l). eapply Hbound.
 Qed.
 
 Theorem fresh_locs_isFresh σg :
   isFresh σg (fresh_locs (dom σg.1.(heap))).
 Proof.
   split.
-  - split.
-    * apply fresh_locs_non_null; auto.
+  - intros. split.
+    * apply fresh_locs_non_null.
     * apply (not_elem_of_dom (D := gset loc)).
-        by apply fresh_locs_fresh.
-  - auto.
+      by apply fresh_locs_fresh.
+  - rewrite /addr_offset /= fresh_locs_off_0 //.
 Qed.
 
 Definition gen_isFresh σg : {l: loc | isFresh σg l}.
@@ -1655,7 +1263,7 @@ Global Instance alloc_gen : GenPred loc (state*global_state) (isFresh) :=
 
 (** Generate a location for a fresh block; doesn't actually insert anything into
 the heap. *)
-Definition allocateN : transition (state*global_state) loc :=
+Definition allocate : transition (state*global_state) loc :=
   suchThat (isFresh).
 
 Global Instance newProphId_gen: GenPred proph_id (state*global_state) (fun '(σ,g) p => p ∉ g.(used_proph_id)).
@@ -1689,146 +1297,92 @@ Definition modifyσ (f : state → state) : transition (state*global_state) () :
 Definition modifyg (f : global_state → global_state) : transition (state*global_state) () :=
   modify (λ '(σ, g), (σ, f g)).
 
-(* Only give semantics to CmpXchg for integers. *)
-Definition val_cmpxchg_safe (v : val) : bool :=
-  match v with
-  | LitV l =>
-      match l with
-      | LitInt _ | LitInt32 _ | LitInt16 _ | LitByte _
-      | LitBool _ | LitLoc _ => true
-      | _ => false
-      end
-  | _ => false
-  end.
-
 Definition go_instruction_step (op : go_instruction) (arg : val) :
   transition (state * global_state) (list observation * expr * list expr) :=
   '(e', s') ← suchThat
     (λ '(σ,g) '(e', s'),
        let _ := σ.(go_state).(go_lctx) in
-       let _ := g.(go_gctx) in
        is_go_step op arg e' σ.(go_state).(package_state) s')
     (gen:=fallback_genPred _);
   modifyσ $ set go_state $ set package_state (λ _, s') ;;
   ret_expr e'.
 
-Definition base_trans (e: expr) :
+Definition base_trans (e : expr) :
  transition (state * global_state) (list observation * expr * list expr) :=
   match e with
   | Rec f x e => atomically $ ret $ RecV f x e
   | Pair (Val v1) (Val v2) => atomically $ ret $ PairV v1 v2
-  | InjL (Val v) => atomically $ ret $ InjLV v
-  | InjR (Val v) => atomically $ ret $ InjRV v
   | App (Val (RecV f x e1)) (Val v2) =>
     ret_expr $ subst' x v2 (subst' f (RecV f x e1) e1)
-  | UnOp op (Val v) => atomically $ unwrap $ un_op_eval op v
-  | BinOp op (Val v1) (Val v2) => atomically $ unwrap $ bin_op_eval op v1 v2
-  | If (Val (LitV (LitBool b))) e1 e2 => ret_expr $ if b then e1 else e2
+  | If (Val v) e1 e2 =>
+       (b ← suchThat (λ _ (b : bool), v = #b) (gen:=fallback_genPred _);
+        ret_expr $ (if (b : bool) then e1 else e2))
   | Fst (Val (PairV v1 v2)) => atomically $ ret v1
   | Snd (Val (PairV v1 v2)) => atomically $ ret v2
-  | Case (Val (InjLV v)) e1 e2 => ret_expr $ App e1 (Val v)
-  | Case (Val (InjRV v)) e1 e2 => ret_expr $ App e2 (Val v)
-  | Fork e => ret ([], Val $ LitV LitUnit, [e])
+  | Fork e => ret ([], Val $ #(), [e])
   (* handled separately *)
-  | Atomically _ _ => undefined
-  | ArbitraryInt =>
+  | ArbitraryInt => atomically (x ← arbitraryInt; ret #x)
+  | Alloc (Val v) =>
     atomically
-      (x ← arbitraryInt;
-      ret $ LitV $ LitInt x)
-  | AllocN (Val (LitV (LitInt n))) (Val v) =>
-    atomically
-      (check (0 < uint.Z n)%Z;;
-       l ← allocateN;
-       modifyσ (state_init_heap l (uint.Z n) v);;
-       ret $ LitV $ LitLoc l)
-   | StartRead (Val (LitV (LitLoc l))) => (* non-atomic load part 1 (used for map accesses) *)
+      (l ← allocate;
+       modifyσ (state_init_heap l v);;
+       ret #l)
+   | StartRead (Val v) => (* non-atomic load part 1 (used for map accesses) *)
      atomically
-       (nav ← reads (λ '(σ,g), σ.(heap) !! l) ≫= unwrap;
+       (l ← suchThat (λ _ (l : loc), v = #l) (gen:=fallback_genPred _);
+        nav ← reads (λ '(σ,g), σ.(heap) !! l) ≫= unwrap;
         match nav with
         | (Reading n, v) =>
-          modifyσ (set heap <[l:=(Reading (S n), v)]>);;
-          ret v
+            modifyσ (set heap <[l:=(Reading (S n), v)]>);;
+            ret v
         | _ => undefined
         end)
-   | FinishRead (Val (LitV (LitLoc l))) => (* non-atomic load part 2 *)
+   | FinishRead (Val v) => (* non-atomic load part 2 *)
      atomically
-       (nav ← reads (λ '(σ,g), σ.(heap) !! l) ≫= unwrap;
+       (l ← suchThat (λ _ (l : loc), v = #l) (gen:=fallback_genPred _);
+        nav ← reads (λ '(σ,g), σ.(heap) !! l) ≫= unwrap;
         match nav with
         | (Reading (S n), v) =>
           modifyσ (set heap <[l:=(Reading n, v)]>);;
-                 ret $ LitV $ LitUnit
+                 ret $ #()
         | _ => undefined
         end)
-   | Load (Val (LitV (LitLoc l))) => (* atomic load (used for most normal Go loads) *)
+   | Load (Val v) => (* atomic load (used for most normal Go loads) *)
      atomically
-       (nav ← reads (λ '(σ,g), σ.(heap) !! l) ≫= unwrap;
+       (l ← suchThat (λ _ (l : loc), v = #l) (gen:=fallback_genPred _);
+        nav ← reads (λ '(σ,g), σ.(heap) !! l) ≫= unwrap;
         match nav with
         | (Reading _, v) => ret v
         | _ => undefined
         end)
-  | PrepareWrite (Val (LitV (LitLoc l))) => (* non-atomic write part 1 *)
+  | PrepareWrite (Val v) => (* non-atomic write part 1 *)
     atomically
-      (v ← (reads (λ '(σ,g), σ.(heap) !! l) ≫= unwrap);
-        match v with
-        | (Reading 0, v) =>
-          modifyσ (set heap <[l:=(Writing, v)]>);;
-          ret $ LitV $ LitUnit
-        | _ => undefined
-        end)
-  | FinishStore (Val (LitV (LitLoc l))) (Val v) => (* non-atomic write part 2 *)
+      (l ← suchThat (λ _ (l : loc), v = #l) (gen:=fallback_genPred _);
+       v ← (reads (λ '(σ,g), σ.(heap) !! l) ≫= unwrap);
+       match v with
+       | (Reading 0, v) =>
+           modifyσ (set heap <[l:=(Writing, v)]>);;
+           ret $ #()
+       | _ => undefined
+       end)
+  | FinishStore (Val vl) (Val v) => (* non-atomic write part 2 *)
     atomically
-      (nav ← reads (λ '(σ,g), σ.(heap) !! l);
+      (l ← suchThat (λ _ (l : loc), vl = #l) (gen:=fallback_genPred _);
+       nav ← reads (λ '(σ,g), σ.(heap) !! l);
        check (is_Writing nav);;
        modifyσ (set heap <[l:=Free v]>);;
-       ret $ LitV $ LitUnit)
-  | AtomicSwap (Val (LitV (LitLoc l))) (Val v) => (* atomic swap *)
-    atomically
-      (nav ← reads (λ '(σ,g), σ.(heap) !! l) ≫= unwrap;
-       match nav with
-       | (Reading 0, v0) =>
-           modifyσ (set heap <[l:=Free v]>);;
-           ret $ v0
-       | _ => undefined
-      end)
-  | AtomicOp op (Val (LitV (LitLoc l))) (Val v) => (* atomic add *)
-    atomically
-      (nav ← reads (λ '(σ,g), σ.(heap) !! l) ≫= unwrap;
-       match nav with
-       | (Reading 0, oldv) =>
-           v ← unwrap (bin_op_eval op oldv v);
-           modifyσ (set heap <[l:=Free v]>);;
-           ret $ v
-       | _ => undefined
-      end)
+       ret $ #() )
   | ExternalOp op (Val v) => atomicallyM $ ffi_step op v
-  | Input (Val (LitV (LitInt selv))) =>
-    atomically
-      (x ← reads (λ '(σ,g), σ.(oracle) σ.(trace) selv);
-      modifyσ (set trace (add_event (In_ev (LitInt selv) (LitInt x))));;
-      ret $ LitV $ LitInt $ x)
-  | Output (Val (LitV v)) =>
-    atomically
-      (modifyσ (set trace (add_event (Out_ev v)));;
-       ret $ LitV $ LitUnit)
   | App (Val (GoInstruction op)) (Val arg) =>
       go_instruction_step op arg
-  | CmpXchg (Val (LitV (LitLoc l))) (Val v1) (Val v2) =>
-    atomically
-      (nav ← reads (λ '(σ,g), σ.(heap) !! l) ≫= unwrap;
-      match nav with
-      | (Reading n, vl) =>
-        check (val_cmpxchg_safe vl || val_cmpxchg_safe v1 = true);;
-        when (vl = v1) (check (n = 0%nat);; modifyσ (set heap <[l:=Free v2]>));;
-        ret $ PairV vl (LitV $ LitBool (bool_decide (vl = v1)))
-      | _ => undefined
-      end)
   | NewProph =>
     atomically
       (p ← newProphId;
        modifyg (set used_proph_id ({[ p ]} ∪.));;
-       ret $ LitV $ LitProphecy p)
-  | ResolveProph (Val (LitV (LitProphecy p))) (Val w) =>
-    ret ([(p, w)], Val $ LitV LitUnit, [])
+       ret $ #p)
+  | ResolveProph (Val pv) (Val w) =>
+      (p ← suchThat (λ _ (p : proph_id), pv = #p) (gen:=fallback_genPred _);
+       ret ([(p, w)], Val $ #(), []))
   | LiteralValue l => atomically $ ret $ LiteralValueV l
   | SelectStmtClauses d cs => atomically $ ret $ SelectStmtClausesV d cs
   | _ => undefined
@@ -1862,31 +1416,6 @@ Definition prim_step'_safe e s g :=
               Fork expressions. *)
   ).
 
-Inductive base_step_atomic:
-    expr -> state -> global_state -> list observation -> expr -> state -> global_state -> list expr -> Prop :=
- | base_step_trans : ∀ e s g κs e' s' g' efs,
-     base_step e s g κs e' s' g' efs →
-     base_step_atomic e s g κs e' s' g' efs
- | base_step_atomically : ∀ (vl : val) e s g κs v' s' g',
-     rtc (λ '(e, (s, g)) '(e', (s', g')), prim_step' e s g [] e' s' g' []) (e, (s, g)) (Val (InjRV v'), (s', g')) →
-     prim_step'_safe e s g →
-     base_step_atomic (Atomically (of_val vl) e) s g κs (Val (InjRV v')) s' g' []
- | base_step_atomically_fail : ∀ vl e s g κs,
-     (* An atomically block can non-deterministically fail _ONLY_ if the block would not trigger UB *)
-     prim_step'_safe e s g →
-     base_step_atomic (Atomically (of_val vl) e) s g κs (Val (InjLV (LitV LitUnit))) s g []
-.
-
-Lemma base_step_atomic_inv e s g κs e' s' g' efs :
-  base_step_atomic e s g κs e' s' g' efs →
-  (∀ el e'', e ≠ Atomically el e'') →
-  base_step e s g κs e' s' g' efs.
-Proof.
-  inversion 1; subst; eauto.
-  - intros. contradiction (H2 (of_val vl) e0); auto.
-  - intros. contradiction (H1 (of_val vl) e0); auto.
-Qed.
-
 (** Basic properties about the language *)
 Global Instance fill_item_inj Ki : Inj (=) (=) (fill_item Ki).
 Proof. induction Ki; intros ???; simplify_eq/=; auto with f_equal. Qed.
@@ -1916,13 +1445,6 @@ Proof.
   simpl in H; eapply suchThat_false; eauto.
 Qed.
 
-Lemma val_base_atomic_stuck e1 σ1 g1 κ e2 σ2 g2 efs :
-  base_step_atomic e1 σ1 g1 κ e2 σ2 g2 efs → to_val e1 = None.
-Proof.
-  inversion 1; subst; eauto using val_base_stuck.
-Qed.
-
-
 Ltac inv_undefined :=
   match goal with
   | [ H: relation.denote (match ?e with | _ => _ end) _ _ _ |- _ ] =>
@@ -1936,17 +1458,6 @@ Proof.
   induction Ki; intros;
     rewrite /base_step /= in H;
     repeat inv_undefined; eauto.
-  - inversion H; subst; clear H. done.
-Qed.
-
-Lemma base_ctx_step_atomic_val Ki e σ1 g1 κ e2 σ2 g2 efs :
-  base_step_atomic (fill_item Ki e) σ1 g1 κ e2 σ2 g2 efs → is_Some (to_val e).
-Proof.
-  inversion 1; subst; eauto using base_ctx_step_val.
-  - destruct Ki; simpl in H0; try solve [ inversion H0 ].
-    inversion H0. subst. eauto.
-  - destruct Ki; simpl in H0; try solve [ inversion H0 ].
-    inversion H0. subst. eauto.
 Qed.
 
 Lemma fill_item_no_val_inj Ki1 Ki2 e1 e2 :
@@ -1957,53 +1468,10 @@ Proof using ext.
   revert Ki1. induction Ki2, Ki1; naive_solver eauto with f_equal.
 Qed.
 
-Lemma alloc_fresh v (n: u64) σ g :
-  let l := fresh_locs (dom σ.(heap)) in
-  (0 < uint.Z n)%Z →
-  base_step_atomic (AllocN ((Val $ LitV $ LitInt $ n)) (Val v)) σ g []
-            (Val $ LitV $ LitLoc l) (state_init_heap l (uint.Z n) v σ) g [].
+Lemma goose_lang_mixin : EctxiLanguageMixin of_val to_val fill_item base_step.
 Proof.
-  intros.
-  constructor 1.
-  rewrite /base_step /=.
-  monad_simpl.
-  eapply relation.bind_runs with (σ,g) l.
-  { econstructor.
-    apply fresh_locs_isFresh.
-  }
-  monad_simpl.
-Qed.
-
-Lemma arbitrary_int_step σ g :
-  base_step_atomic (ArbitraryInt) σ g []
-            (Val $ LitV $ LitInt $ W64 0) σ g [].
-Proof.
-  intros.
-  constructor 1.
-  rewrite /base_step /=.
-  monad_simpl.
-  eapply relation.bind_runs; [ | monad_simpl ].
-  constructor; auto.
-Qed.
-
-Lemma new_proph_id_fresh σ g :
-  let p := fresh g.(used_proph_id) in
-  base_step_atomic NewProph σ g [] (Val $ LitV $ LitProphecy p) σ (set used_proph_id ({[ p ]} ∪.) g) [].
-Proof.
-  intro p.
-  constructor 1.
-  rewrite /base_step /=.
-  monad_simpl.
-  eapply relation.bind_runs with (σ,g) p.
-  { econstructor.
-    apply is_fresh. }
-  monad_simpl.
-Qed.
-
-Lemma goose_lang_mixin : EctxiLanguageMixin of_val to_val fill_item base_step_atomic.
-Proof.
-  split; apply _ || eauto using to_of_val, of_to_val, val_base_atomic_stuck,
-    fill_item_val, fill_item_val_inv, fill_item_no_val_inj, base_ctx_step_atomic_val.
+  split; apply _ || eauto using to_of_val, of_to_val, val_base_stuck,
+    fill_item_val, fill_item_val_inv, fill_item_no_val_inj, base_ctx_step_val.
 Qed.
 
 End external.
@@ -2013,10 +1481,10 @@ Global Notation zero_val := zero_val_def.
 (** Language *)
 
 Arguments ffi_semantics ext ffi : clear implicits.
-Arguments goose_lang_mixin {ext} {ffi} ffi_semantics.
+Arguments goose_lang_mixin {ext} {ffi} {go_gctx} ffi_semantics.
 
 Section goose.
-  Context {ext: ffi_syntax} {ffi: ffi_model}
+  Context {ext: ffi_syntax} {ffi: ffi_model} {go_goctx : GoGlobalContext}
           {ffi_semantics: ffi_semantics ext ffi}.
   Canonical Structure goose_ectxi_lang := (EctxiLanguage (goose_lang_mixin ffi_semantics)).
   Canonical Structure goose_ectx_lang := (EctxLanguageOfEctxi goose_ectxi_lang).
@@ -2041,21 +1509,11 @@ Proof.
   by simplify_eq.
 Qed.
 
-Lemma prim_step_to_val_is_base_step e σ1 g1 κs w σ2 g2 efs :
-  prim_step e σ1 g1 κs (Val w) σ2 g2 efs → base_step_atomic (ffi_semantics:=ffi_semantics) e σ1 g1 κs (Val w) σ2 g2 efs.
-Proof.
-  intro H. destruct H as [K e1 e2 H1 H2].
-  assert (to_val (fill K e2) = Some w) as H3; first by rewrite -H2.
-  apply to_val_fill_some in H3 as [-> ->]. subst e. done.
-Qed.
-
 Lemma base_prim_step_trans e σ g κ e' σ' g' efs :
   base_step e σ g κ e' σ' g' efs →
   ectx_language.prim_step e σ g κ e' σ' g' efs.
 Proof.
-  intros.
-  apply base_prim_step. apply base_step_trans.
-  auto.
+  intros. apply base_prim_step. auto.
 Qed.
 
 Lemma base_prim_step_trans' e σ g κ e' σ' g' efs :
@@ -2132,7 +1590,6 @@ Proof.
     by exists (comp_ectx K K') e1' e2'; rewrite ?Heq1 ?Heq2 ?fill_comp.
   - intros e1 σ1 g1 κ e2 σ2 g2 efs Hnval [K'' e1'' e2'' Heq1 -> Hstep].
     destruct (step_by_val K K'' e1 e1'' σ1 g1 κ e2'' σ2 g2 efs) as [K' ->]; eauto.
-    { econstructor. eauto. }
     rewrite -fill_comp' in Heq1; apply (inj (fill _)) in Heq1.
     exists (fill K' e2''); rewrite -fill_comp'; split; auto.
     econstructor; eauto.
@@ -2170,12 +1627,6 @@ Proof.
     apply fill_step_inv' in Hstep; eauto.
     naive_solver.
 Qed.
-
-Definition trace_observable e r σ g tr :=
-  ∃ σ2 g2 t2 stat, erased_rsteps (CS:=goose_crash_lang) r ([e], (σ, g)) (t2, (σ2, g2)) stat ∧ σ2.(trace) = tr.
-
-Definition trace_prefix (tr: Trace) (tr': Trace) : Prop :=
-  prefix tr tr'.
 
 Lemma ExternalOp_fill_inv K o e1 e2:
   ExternalOp o e1 = fill K e2 →
@@ -2266,33 +1717,8 @@ Proof.
   split; first done.
   apply prim_base_irreducible; auto.
   * inversion 1; subst; eauto.
-    inversion H0; auto.
   * intros Hval. apply ectxi_language_sub_redexes_are_values => Ki e' Heq.
     apply Panic_fill_item_inv in Heq; subst; auto; by exfalso.
-Qed.
-
-Lemma atomically_not_stuck_body_safe (l: val) e σ g :
-  ¬ stuck (Atomically (of_val l) e) σ g →
-  prim_step'_safe e σ g.
-Proof.
-  intros Hnstuck ??? Hrtc Hstuck.
-  apply Hnstuck.
-  split; first done.
-  apply prim_base_irreducible; last first.
-  { intros Hval. apply ectxi_language_sub_redexes_are_values => Ki e0' Heq.
-    assert (of_val l = e0').
-    { move: Heq. destruct Ki => //=; congruence. }
-    naive_solver.
-  }
-  intros ????? Hstep.
-  inversion Hstep; subst.
-  * inversion H; eauto.
-  * match goal with
-    | [ H: prim_step'_safe _ _ _ |- _ ] => eapply H
-    end; try eapply Hrtc; eauto.
-  * match goal with
-    | [ H: prim_step'_safe _ _ _ |- _ ] => eapply H
-    end; eauto.
 Qed.
 
 Definition null_non_alloc {V} (h : gmap loc V) :=
