new/proof/proof_prelude.v
@@ -1,7 +1,7 @@
 From iris.algebra Require Export auth gmap frac agree excl vector.
 From Perennial.algebra Require Export big_op.
 From Perennial.Helpers Require Export
-  Tactics List ListLen Transitions ModArith iris ipm.
+  Tactics List ListLen Transitions ModArith iris ipm Integers.
 From Perennial.base_logic Require Export ghost_var.
 From Perennial.program_logic Require Export ncinv.
 From Perennial Require Export base.
